

Recitation #1

$$P \vee (q \wedge r) \vee (r \wedge p)$$

↓ when making truth table

Left-Right

go left to right in columns

P	(q ∧ r)	(r ∧ p)
.	,	.
.	,	,

... telling the truth, he's a knave
... then he's telling the truth

If he's telling the truth
If he's a knave

CS 2050 Worksheet 1

G: gawain is a knight
B: Bedivere is a knight

1.2 Truth Table

- a) You are on an island of knights and knaves, where knights always tell the truth and knaves always lie. You encounter two people Gawain and Bedivere. Gawain says "I am a knave or Bedivere is a knight" and Bedivere says nothing. Determine, if possible, what Gawain and Bedivere are.

G	B	$\neg G \vee B$	$\neg G \vee B \rightarrow G$	$G \rightarrow (\neg G \vee B)$	$\neg G \vee B \leftrightarrow G$
T	T	T	T	F	T
T	F	F	T	F	F
F	T	T	F	T	F
F	F	F	F	T	F

So both are knights

- b) Build a truth table to show that for some propositions p, q and r: $q \wedge \neg p \rightarrow r$ and $q \rightarrow (\neg p \rightarrow r)$ are equivalent.

P	q	r	$\neg p$	$\neg p \rightarrow r$	$q \wedge \neg p$	$q \wedge \neg p \rightarrow r$	$q \rightarrow (\neg p \rightarrow r)$	$q \wedge \neg p \rightarrow r \equiv q \rightarrow (\neg p \rightarrow r)$
T	T	T	F	T	T	T	T	T
T	T	F	F	F	T	F	F	F
T	F	T	F	T	F	T	T	T
T	F	F	F	T	F	T	T	T
F	T	T	T	T	T	T	T	T
F	T	F	T	F	T	F	F	F
F	F	T	T	T	F	T	T	T
F	F	F	T	T	F	T	T	T

order of precedence

Conclusion: since the propositions ... is true

equiv

1.3 Logical Equivalences

- a) Use only logical equivalences and material implication to prove that $p \rightarrow q$ is equivalent to its contrapositive, $\neg q \rightarrow \neg p$.

STUDY

- 1) $p \rightarrow q$
 2) $\neg p \vee q$
 3) $q \vee \neg p$
 4) $\neg(\neg q) \vee \neg p$
 5) $\neg q \rightarrow \neg p$
- material implication
 LHS
 material implication
 commutative
 double negative
 material implication

Conclusion: using logical equiv. I have shown that $p \rightarrow q = \neg q \rightarrow \neg p$

$$(\overline{p} + \overline{q}) + p$$

b) Use only logical equivalences and material implication to show whether or not $(p \wedge q) \rightarrow p$ is a tautology.

$$\neg p \vee q$$

$$(p \wedge q) \rightarrow p$$

$$\neg(p \wedge q) \vee p$$

material implication

$$(\neg p \vee \neg q) \vee p$$

De Morgan's

$$(\neg p \vee p) \vee \neg q$$

commutative

$$T \vee \neg q$$

negation

$$\neg q \vee T$$

commutative

$$T$$

domination

~~T~~ must be on RHS

Concl: using logical equiv. I have shown this statement is a tautology.

c) Use only logical equivalences and material implication to show that $q \wedge \neg p \rightarrow r$ is equivalent to $q \rightarrow (\neg p \rightarrow r)$.

$$\text{Prove } q \wedge \neg p \rightarrow r \equiv q \rightarrow (\neg p \rightarrow r)$$

$$\overline{q} + p + r$$

$$q \wedge \neg p \rightarrow r$$

LHS

$$\neg(q \wedge \neg p) \vee r$$

material implication

$$(\neg q \vee \neg(\neg p)) \vee r$$

De Morgan's

$$(\neg q \vee p) \vee r$$

double negation

$$\neg q \vee (p \vee r)$$

commutative

$$\neg q \vee (\neg(\neg p) \vee r)$$

double neg.

$$\neg q \vee (\neg p \rightarrow r)$$

material imp

$$q \rightarrow (\neg p \rightarrow r)$$

material imp

Thus, Concl. by logical equiv., the proposition $q \wedge \neg p \rightarrow r$ is equiv. to the proposition $q \rightarrow (\neg p \rightarrow r)$.

$A \wedge B$
 \uparrow
 A says "The two of us are both knights" and
 B says "A is a knave"
 $\hookrightarrow \neg A$

$$(A \wedge B \rightarrow A) \quad (A \rightarrow A \wedge B)$$

$$(\neg A \rightarrow B) \quad (B \rightarrow \neg A)$$

A	B	$A \wedge B$	$A \wedge B \rightarrow A$	$A \rightarrow A \wedge B$	$A \wedge B \leftrightarrow A$	$\neg A$	$\neg A \rightarrow B$	$B \rightarrow \neg A$	$\neg A \leftrightarrow B$
T	T	T	T	T	T	F	T	F	F
T	F	F	T	F	F	F	T	T	T
F	T	F	T	T	<u>T</u>	T	T	T	<u>T</u>
F	F	F	T	T	T	T	F	T	F

A is a knave

B is a knight

$A \quad B$
 $\uparrow \quad \uparrow$
 Both A and B say "I am a knight."

$$A \rightarrow A$$

$$B \rightarrow B$$

A	B	$A \rightarrow A$	$B \rightarrow B$	$A \leftrightarrow A$	$B \leftrightarrow B$
T	T	T	T	T	T
T	F	T	T	T	T
F	T	T	T	T	T
F	F	T	T	T	T

$$\exists x (\forall y (x \neq y \rightarrow (\neg E(y, x) \vee \neg T(y, x))))$$

for all students in class, x uses snapchat or there exists y that uses snapchat and x and y are friends.

For all students in the class, they either use snapchat or someone else exists who uses snapchat and are friends with the original.

there exists a student x and student y for all classes they are distinct students and student x has taken all z classes if and only if student y has taken all z classes.

01

ar